doc: exploring some different approaches

Grw/TestsGrewrite.lean
@@ -6,11 +6,17 @@ section Examples
 set_option trace.Meta.Tactic.grewrite true
 set_option trace.Meta.Tactic.eauto true
 set_option trace.Meta.Tactic.eauto.hints true
+set_option trace.Meta.Tactic.eauto.goals true
+set_option trace.Meta.Tactic.eauto.instances true
 
 -- ATOM
-example {r : relation Prop} [Subrel r (flip impl)] : r a b → b → a := by
+example {r : relation Prop} [hp : Proper (r ⟹ Iff) id] : r a b → b → a := by
   intro rab hb
   grewrite [rab]
+  exact hb
+  constructor
+  have hp' := hp.proper
+  rw [respectful] at hp'
   exact hb
 
 -- Simple app
@@ -49,6 +55,8 @@ variable [Proper_Pα: Proper (Rα ⟹ Iff) Pα]
 variable [PER Rα] [PER Rβ]
 
 -- Smallest example
+-- Coq TC:
+#check Proper (r ⟹ flip impl) Pα
 example (h: Rα a a') (finish: Pα a') : Pα a := by
   grewrite [h]
   exact finish
@@ -75,7 +83,43 @@ example (h: Rα a a') (finish: Rα a' a'): Rα a a := by
 example (h: Rα a a') (finish: Pα a'): Pα a ∧ Pα a ∧ Pα a ∧ Pα a ∧ Pα a ∧ Pα a := by
   sorry
 
+example : ∀ P Q : Prop, (P ↔ Q) → (Q → P ) := by
+  intros P Q H
+  grewrite [H]
+  . simp [impl]
+  . exact (flip impl)
+  . constructor
+    intros
+    assumption
+  . exact (flip impl) ⟹ Iff
+  . constructor
+    intros f g h
+    rw [respectful] at *
+    aesop
+    specialize h x x
+    rw [flip, impl] at *
+    aesop
+  . exact impl ⟹ flip impl ⟹ Iff
+  . exact Iff
+  . have inner := Subrel.subrelation impl impl (Proper.mk Q Q)
+    apply (Subrel.subrelation (impl Q) (impl Q) (Subrel.subrelation impl impl Proper.proper Q Q Proper.proper) P Q H)
+    sorry
+  . sorry
+  . sorry
+--Proof: Subrel.subrelation (impl Q) (impl Q) (Subrel.subrelation impl impl Proper.proper Q Q Proper.proper) P Q H
+
 -- Examples from the Paper
+inductive ex {A : Sort u} (P : A → Prop) : Prop
+  | intro : ∀ x : A, P x → ex P
+
+example {A : Sort u} {P Q : A → Sort v} [Proper (pointwiseRelation A <| iff ⟹ iff) (@ex A)] : ∀A P Q, (∀ x : A, P x ↔ Q x) → (∃x:A, ¬Q x) → (∃x:A, ¬P x) := by
+  sorry
+
+example : ∀ P Q : Prop, (P ↔ Q) → (Q → P ) ∧ (Q → P ) := by
+  intros P Q H
+  grewrite [H]
+  simp
+
 variable {SET : Type}
 variable {eqset : relation SET}
 def trueRelation (α : Type) : relation α := fun _ _ => True
@@ -99,3 +143,95 @@ example : ∀ s, eqset (union (union s empty) s) s := by
   apply Reflexive.rfl
 
 end Examples
+
+/-
+Some Coq constraints for problems:
+-/
+
+-- Produces: Subrel Iff (flip impl)
+example : ∀ P Q : Prop, (P ↔ Q) → Q → P := by
+  intros P Q H HQ
+  grewrite [H]
+  exact HQ
+
+--Produces: Proper (r ⟹ flip impl) P
+example {r : relation α} {P : α → Prop} [Proper (r ⟹ Iff) P] : r a a' → P a' → P a := by
+  intros h finish
+  grewrite [h]
+  exact finish
+
+/-
+Produces wrt. to subrelationProper and do_subrelation:
+  ?m1 : Relation A
+  ?m2 : Proper (r ==> ?m1) f
+  ?m3 : Proper (r ==> flip impl) P
+-/
+example {f : α → α} [Proper (r ⟹ r) f] [Proper (r ⟹ Iff) P] : r a a' → P (f a') → P (f a) := by
+  intro h finish
+  grewrite [h]
+  exact finish
+
+/-
+Produces: Nothing to rewrite.
+-/
+-- RW under lambda
+example {a : α} {P : (α → α) → Prop} [Proper (pointwiseRelation α r ⟹ Iff) P] : r a a' → P (λ _ => a') → P (λ _ => a) := by
+  intro h finish
+  grewrite [h]
+  exact finish
+
+/-
+Produces: wrt. to subrelationProper and do_subrelation:
+  ?m1 : Proper (Iff ==> flip impl) (impl Q)
+-/
+example : ∀ P Q : Prop, (P ↔ Q) → (Q → P):= by
+  intros P Q H
+  grewrite [H]
+  simp
+
+/-
+Produces: wrt. to subrelationProper and do_subrelation:
+  ?m1 : Proper (Iff ==> flip impl) (impl Q)
+-/
+example : ∀ P Q : Prop, (P ↔ Q) → (Q → P) := by
+  intros P Q H
+  grewrite [H]
+  simp
+
+/-
+Produces: wrt. to subrelationProper and do_subrelation:
+  ?m1 : Proper (?r ==> ?r0 ==> flip impl) impl
+  ?m2 : Proper (iff ==> ?r0) (impl Q)
+  ?r : Relation Prop
+  ?m3 : Proper (Iff => ?r) (impl Q)
+  ?r0 : Relation Prop
+-/
+example : ∀ P Q : Prop, (P ↔ Q) → (Q → P) → (Q → P) := by
+  intros P Q H
+  grewrite [H]
+  simp
+
+/-
+Produces: wrt. to subrelationProper and do_subrelation:
+  ?m1 : Proper (?r ==> ?r0 ==> flip impl) and
+  ?m2 : Proper (iff ==> ?r0) (impl Q)
+  ?r : Relation Prop
+  ?m3 : Proper (Iff => ?r) (impl Q)
+  ?r0 : Relation Prop
+-/
+example : ∀ P Q : Prop, (P ↔ Q) → (Q → P) ∧ (Q → P) := by
+  intros P Q H
+  grewrite [H]
+  simp
+
+/-
+Produces: wrt. to subrelationProper and do_subrelation:
+  ?m1 : ProperProxy ?r0 (Q -> Q)
+  ?m2 : Proper (?r ==> ?r0 ==> flip impl) And
+  ?m3 : Proper (Iff ==> ?r) (impl Q)
+  ?r : Relation Prop
+-/
+example : ∀ P Q : Prop, (P ↔ Q) → (Q → P) ∧ (Q → Q) := by
+  intros P Q H
+  grewrite [H]
+  simp
